src/lib/notation.lean
@@ -1,0 +1,98 @@
+import tactic
+
+universes u
+
+@[notation_class] class has_succ (α : Sort*) := (succ : α → α)
+
+prefix `Succ `:85 := has_succ.succ
+
+def numeral {α : Type*} [has_zero α] [has_succ α] : ℕ → α
+| 0       := 0
+| (n + 1) := Succ (numeral n)
+
+instance numeral_has_one {α : Type*} [has_zero α] [has_succ α] : has_one α := ⟨Succ 0⟩
+
+lemma numeral_one_def  {α : Type*} [has_zero α] [has_succ α] : (1 : α) = Succ 0 := rfl 
+
+@[notation_class] class has_eq (α : out_param (Sort*)) (β : Sort*) := (eq : α → α → β)
+
+infix ` ≃ `:50 := has_eq.eq
+
+@[notation_class] class has_preceq (α : out_param (Sort*)) (β : Sort*) := (preceq : α → α → β)
+
+infix ` ≼ `:50 := has_preceq.preceq
+
+@[notation_class] class has_elem (α : out_param (Sort*)) (β : Sort*) := (elem : α → α → β)
+
+infix ` ∊ `:50 := has_elem.elem
+
+@[notation_class] class has_negation (α : Sort*) := (neg : α → α)
+
+prefix `⁻`:75 := has_negation.neg
+
+@[reducible] def has_eq.ineq {α : out_param (Sort*)} {β : Sort*} [has_eq α β] [has_negation β] (a b : α) : β := ⁻(a ≃ b)
+
+infix ` ≄ `:50 := has_eq.ineq
+
+@[notation_class] class has_arrow (α : Sort*) := (arrow : α → α → α)
+
+infixr ` ⟶ `:60 := has_arrow.arrow
+
+@[notation_class] class has_lrarrow (α : Sort*) := (lrarrow : α → α → α)
+
+@[notation_class] class has_univ_quantifier (α : Sort*) := (univ : α → α)
+
+prefix `∏ `:64 := has_univ_quantifier.univ
+
+@[notation_class] class has_exists_quantifier (α : Sort*) := (ex : α → α)
+
+prefix `∐ `:64 := has_exists_quantifier.ex
+
+@[notation_class] class has_univ_quantifier' (α : Sort*) (β : Sort*):= (univ : α → β)
+
+prefix `∏' `:64 := has_univ_quantifier'.univ
+
+@[notation_class] class has_exists_quantifier' (α : Sort*) (β : Sort*) := (ex : α → β)
+
+prefix `∐' `:64 := has_exists_quantifier'.ex
+
+@[notation_class] class has_turnstile (α : Sort*) := (turnstile : set α → α → Prop)
+
+infix ` ⊢ `:45 := has_turnstile.turnstile
+notation T ` ⊢{`:45 β `} `:45 p := has_turnstile.turnstile T β p
+
+namespace has_turnstile
+variables {α : Type*} [has_turnstile α]
+
+def turnstile_set (T : set α) (Γ : set α) : Prop := ∀ p ∈ Γ, T ⊢ p
+
+infix ` ⊢* `:45 := turnstile_set
+
+end has_turnstile
+
+@[notation_class] class has_Longarrow (α : Sort*) := (Longarrow : set α → α → Type u)
+
+infix ` ⟹ `:45 := has_Longarrow.Longarrow
+
+def has_arrow.lrarrow {α : Type*} [has_arrow α] [has_inf α] (a b : α) : α := (a ⟶ b) ⊓ (b ⟶ a)
+
+infix ` ⟷ `:59 := has_arrow.lrarrow
+
+lemma lrarrow_def {α : Type*} [has_arrow α] [has_inf α] (a b : α) : a ⟷ b = (a ⟶ b) ⊓ (b ⟶ a) := rfl
+
+@[notation_class] class has_double_turnstile (α : Sort*) (β : Sort*) := (double_turnstile : α → β → Prop)
+
+infix ` ⊧ ` :55 := has_double_turnstile.double_turnstile
+
+namespace has_double_turnstile
+variables {α : Type*} {β : Type*} [has_double_turnstile α β]
+
+def double_turnstile_set (T : α) (S : set β) : Prop := ∀ p ∈ S, T ⊧ p
+
+infix ` ⊧* `:45 := double_turnstile_set
+
+end has_double_turnstile
+
+class has_logic_symbol (F : Sort*)
+  extends has_negation F, has_arrow F, has_inf F, has_sup F, has_top F, has_bot F
+
